Attempt with inductive Context
Signed-off-by: Gavin Zhao <gavinz@brown.edu>

Ltlc/Basic.lean
@@ -16,35 +16,48 @@ inductive LtlcTerm
   | app : LtlcTerm → LtlcTerm → LtlcTerm
   deriving Repr, BEq
 
-def Context := AssocList String LtlcType
+-- /- def Context := AssocList String LtlcType -/
+-- /--/
+-- /- instance : Membership String (AssocList String LtlcType) where -/
+-- /-   mem l x := l.contains x = true -/
+-- /--/
+-- /- instance : Membership String Context where -/
+-- /-   mem l x := l.contains x = true -/
+-- /--/
+-- /- def context_append (x y : Context) : Context := -/
+-- /-     match y with  -/
+-- /-     | .nil => x  -/
+-- /-     | .cons k v ys => .cons k v (context_append x ys) -/
+-- /--/
+-- /- instance : Append Context where -/
+-- /-   append x y := context_append x y -/
 
-instance : Membership String (AssocList String LtlcType) where
+inductive Context 
+  | empty : Context 
+  | single : String → LtlcType → Context 
+  | combine : Context → Context → Context
+
+def Context.contains (c : Context) (x : String) : Bool :=
+  match c with 
+  | .empty => false 
+  | .single y _ => x = y 
+  | .combine l r => l.contains x || r.contains x
+
+instance : Membership String Context where 
   mem l x := l.contains x = true
-
-instance : Membership String Context where
-  mem l x := l.contains x = true
-
-def context_append (x y : Context) : Context :=
-    match y with 
-    | .cons k v ys => context_append (AssocList.cons k v x) ys
-    | .nil => x
-
-instance : Append Context where
-  append x y := context_append x y
-
 
 inductive HasType : Context → LtlcTerm → LtlcType → Prop
-  | var {x τ} : HasType (AssocList.cons x τ AssocList.empty) (.var x) τ
+  | var {x τ} : HasType (.single x τ) (.var x) τ
   | lam 
     {Γ x α β body}
     (x_fresh : x ∉ Γ)
-    (v_hastype : HasType (AssocList.cons x α Γ) body β)
+    (v_hastype : HasType (Γ.combine (.single x α)) body β)
     : HasType Γ (LtlcTerm.lam x α body) (.arrow α β)
   | app 
     {Γ₁ Γ₂ t u α β}
     (t_is_fn : HasType Γ₁ t (.arrow α β))
     (u_is_α : HasType Γ₂ u α)
-    : HasType (Γ₁ ++ Γ₂) (.app t u) β
+    : HasType (Γ₁.combine Γ₂) (.app t u) β
 
 @[simp]
 def subst (x : String) (e : LtlcTerm) (a : LtlcTerm) : LtlcTerm := 
@@ -63,23 +76,23 @@ inductive Step : LtlcTerm → LtlcTerm → Prop
     : Step e₁ e₂ → Step (.app f e₁) (.app f e₂)
 
 theorem subst_preserves_type {Γ₁ Γ₂ x α β e a} 
-  (p1 : HasType (Γ₁.cons x α) e β)
+  (p1 : HasType (.combine Γ₁ (.single x α)) e β)
   (p2 : HasType Γ₂ a α)
-  : HasType (Γ₁ ++ Γ₂) ([x // a] e) β :=  sorry
+  : HasType (.combine Γ₁ Γ₂) ([x // a] e) β :=
     /- match p1 with  -/
-    /- | .var => _ -/
     /- | .lam b x => _ -/
     /- | @HasType.app a b c d e f g h => _ -/
-    /- match e with  -/
-    /- | .var y =>  -/
-    /-       /- by  -/ -/
-    /-       /-   by_cases heq : y = x  -/ -/
-    /-       /-   . simp [heq] -/ -/
-    /-       /-     _ -/ -/
-    /-       /-   . simp [heq] -/ -/
-    /-       /-     _ -/ -/
-    /- | .lam z γ b => _  -/
-    /- | .app f u => _ -/
+    match e with 
+    | .var y => 
+        by 
+          by_cases heq : y = x 
+          . simp [heq]
+            rw [heq] at p1 
+            _
+          . simp [heq]
+            contradiction
+    | .lam z γ b => _ 
+    | .app f u => _
 
 theorem preservation {Γ τ e₁ e₂}
   (e₁_is_τ : HasType Γ e₁ τ)
